nola/examples/rust_halt/shrref.v
@@ -38,14 +38,15 @@ Section ty_shrref.
   Qed.
 
   (** [ty_shrref] satisfies [TyOp] *)
-  #[export] Instance ty_shrref_ty_op `{!Ty (X:=X) T sz, !TyOpLt T α d} {β} :
-    α ⊑ β → TyOpAt (ty_shrref β T) α d.
+  #[export] Instance ty_shrref_ty_op
+    `{!Ty (X:=X) T sz, !TyOpLt T α d, !LftIncl α β} :
+    TyOpAt (ty_shrref β T) α d.
   Proof.
-    move=> ?. apply: sty_op_at=> >. rewrite sty_shrref_unseal /=.
+    apply: sty_op_at=> >. rewrite sty_shrref_unseal /=.
     iIntros "α". iDestruct 1 as (??? -> ??) "#T". rewrite sem_cif_in /=.
     iMod (stored_acc with "T") as "{T}T".
     iDestruct (lft_incl_live_acc (β:=α ⊓ β) with "α") as (?) "[αβ →α]".
-    { by apply lft_incl_meet_intro. }
+    { exact lft_incl'. }
     iMod (ty_shr_proph_lt with "αβ T") as (???) "[$ →T]"=>//. iModIntro.
     iSplit. { iPureIntro. by eapply proph_dep_proper. }
     iIntros "ξl". iMod ("→T" with "ξl") as "[αβ T]".
@@ -82,13 +83,13 @@ Section ty_shrref.
   Qed.
 
   (** Read a copyable object from [ty_shrref] *)
-  Lemma read_ty_shrref `{!Ty (X:=X) T sz, !Copy T sz} {α β} :
-    α ⊑□ β ⊢ read α (ty_shrref β T) T (ty_shrref β T) id id.
+  Lemma read_ty_shrref `{!Ty (X:=X) T sz, !Copy T sz, !LftIncl α β} :
+    ⊢ read α (ty_shrref β T) T (ty_shrref β T) id id.
   Proof.
-    rewrite read_unseal. iIntros "#⊑" (?????) "!>/= α t".
+    rewrite read_unseal. iIntros (?????) "!>/= α t".
     rewrite sty_shrref_unseal /=. iDestruct 1 as (???[= ->]??) "#sT".
     rewrite sem_cif_in /=. iMod (stored_acc with "sT") as "sT'".
-    iMod (lft_sincl_live_acc with "⊑ α") as (?) "[β →α]".
+    iDestruct (lft_incl_live_acc with "α") as (?) "[β →α]"=>//.
     iMod (copy_shr_acc with "β t sT'") as (??) "(↦ & t & #T & cl)"=>//.
     iModIntro. iDestruct (ty_own_clair with "T") as "$"=>//. iFrame "↦".
     iSplit=>//. iIntros "↦". iMod ("cl" with "↦ t") as "[β $]". iModIntro.
